\begin{remark}[Notation]
    Let $X$ and $G$ be graphs. Let $\mathbb{F}$ be a finite set of monomorphisms with $dom(f) \mathop{=} X$ for all $f \mathop{\in} \mathbb{F}$. We define
    \begin{align*}
        \operatorname{Mono}(X-\mathbb{F},G) \mathop{=} \{ \iota \mathop{\in} \operatorname{Mono}(X,G) \ | \ \forall f \mathop{\in} \mathbb{F}. \nexists \beta \mathop{\in} \operatorname{Mono}(codom(f),G).~\iota \mathop{=} f \mathop{\star} \beta \} 
        \\
        \operatorname{Mono}(X,G,\alpha) \mathop{=} \{ \iota \mathop{\in} \operatorname{Mono}(X,G) \ | \ \exists \beta : X \mathop{\to} A.~\iota \mathop{=} \beta \mathop{\star} \alpha \} 
        \\
        \operatorname{Mono}(X,G,\lnot \alpha) \mathop{=} \{ \iota \mathop{\in} \operatorname{Mono}(X,G) \ | \ \nexists \beta : X \mathop{\to} A.  ~\iota \mathop{=} \beta \mathop{\star} \alpha \} 
        \\
        \operatorname{Mono}(X,G, \lnot \alpha, \beta) \mathop{=} \{ 
            \iota \mathop{\in}  \operatorname{Mono}(X,G) \ | \ (\nexists \zeta. ~\iota \mathop{=} \zeta \mathop{\star} \beta') \mathop{\land} (\exists \zeta.~\iota \mathop{=} \zeta \mathop{\star} \alpha')
        \}
        \\
        \operatorname{Mono}(X,G,\lnot \alpha, \lnot \beta) \mathop{=} \{ 
            \iota \mathop{\in} \operatorname{Mono}(X,G) \ | \ (\nexists \zeta. ~\iota \mathop{=} \zeta \mathop{\star} \beta') \mathop{\land} (\nexists \zeta.~\iota \mathop{=} \zeta \mathop{\star} \alpha')
        \}
        \end{align*}
\end{remark}

\begin{definition}[Non-decreasing Rule]
    Let $X$ be a graph and $L \overset{l}{\leftarrowtail} K \overset{r}{\rightarrowtail} R$ a linear DPO rewriting rule. We say that the rule is $X$-non-decreasing if the rule 
    $R \overset{r}{\leftarrowtail} K \overset{l}{\rightarrowtail} L$ is $X$-non-increasing. 
\end{definition}

\begin{theorem}
    \label{thm:termination_grs_ext1} 
    Let \(\mathcal{A}\) and \(\mathcal{B}\) be sets of linear DPO rewriting rules. If there is a graph \(X\) and a monomorphism $h: X \rightarrowtail F$ such that
    \begin{itemize}
        \item for every rule $\rho \mathop{\in} \mathcal{A} \mathop{\cup} \mathcal{B}$, the rule $\rho$ is $X$-non-increasing,
        \item for every rule $\rho \mathop{\in} \mathcal{A} \mathop{\cup} \mathcal{B}$, the rule $\rho^{-1}$ is $X$-non-increasing,
        \item for every rule \(\rho \mathop{\in} \mathcal{A} \mathop{\cup} \mathcal{B}\), the rule $\rho^{-1}$ is $F$-non-increasing,
        \item for all subgraph $K'$ of $K$, if there is an occurrence of $F$ in $G$ around $K'$, then there is an occurrence of $F$ in $H$ around $K'$,
        \item For every rule \(\left( L \overset{l}{\leftarrowtail} K \overset{r}{\rightarrowtail} R \right) \mathop{\in} \mathcal{A}\), we have \(|\operatorname{Mono}(X-F,L)| \mathop{>} |\operatorname{Mono}(X-F,R)|\),
        \item For every rule \(\left( L \overset{l}{\leftarrowtail} K \overset{r}{\rightarrowtail} R \right) \mathop{\in} \mathcal{B}\), we have \(|\operatorname{Mono}(X-F,L)| \mathop{\geq} |\operatorname{Mono}(X-F,R)|\),
    
    \end{itemize}
    then \(\mathop{\Rightarrow}_{\mathcal{A},\mathcal{M}}\) is terminating relative to \(\mathop{\Rightarrow}_{\mathcal{B},\mathcal{M}}\).
\end{theorem}



\begin{flalign*}
    &\card{Mono(X- F, G)} - \card{Mono(X- F, H)} \\
   =&\card{Mono(X- F, G, l') \uplus Mono(X- F, G, \lnot l', m) \uplus Mono(X- F, G, \lnot l', \lnot m)} - \\ 
      &\card{Mono(X- F, H, r') \uplus Mono(X- F, G, \lnot r', m') \uplus Mono(X- F, H, \lnot r', \lnot m')} \\
   =&\left( | Mono(X- F, G, l')|\mathop{+}|Mono(X- F, G, \lnot l', m)|+ |Mono(X- F, G, \lnot l', \lnot m)|\right) - \\ 
    &\left(|Mono(X- F, H, r')|\mathop{+}|Mono(X- F, H, \lnot r', m')|\mathop{+}|Mono(X- F, H, \lnot r', \lnot m')|\right)\\
    \mathop{=} &\left( | Mono(X- F, G, l')| - |Mono(X- F, H, r')| \right)\mathop{+}\\
    &\left( |Mono(X- F, G, \lnot l', m)| - |Mono(X- F, G, \lnot l', \lnot m)|\right)\mathop{+}\\ 
    &\left( |Mono(X- F, H, \lnot r', \lnot m')| - |Mono(X- F, H, \lnot r', m')|\right) \\
    & \text{because $| Mono(X- F, G, l')| \mathop{=} |Mono(X- F, H, r')|$} \\
    \mathop{=} &\left( | Mono(X- F, G, l')| - |Mono(X- F, H, r')| \right)\mathop{+}\\
    &\left( |Mono(X- F, G, \lnot l', m)| - |Mono(X- F, G, \lnot l', \lnot m)|\right)\mathop{+}\\ 
    &\left( |Mono(X- F, H, \lnot r', \lnot m')| - |Mono(X- F, H, \lnot r', m')|\right)
\end{flalign*}

\begin{proposition}
    $| Mono(X- F, G, l')| - |Mono(X- F, H, r')| \mathop{\geq} 0$
\end{proposition}
\begin{proof}
    \begin{flalign}
        &|Mono(X- F, G, l')| - |Mono(X- F, H, r')| \\
        =&(|Mono(X, G, l')| - | Mono(X\mathop{+}F, G, l')|)-\\
        & (|Mono(X, H, r')| - |Mono(X+ F, H, r')|) \\
        =&(|Mono(X, G, l')| - | Mono(X, H, r')|)+(|Mono(X+ F, H, r')| - |Mono(X+ F, G, l')|) \\
        \mathop{\geq} &(|Mono(X+ F, H, r')| - |Mono(X+ F, G, l')|) 
        \\
        &\text{because $|Mono(X, G, l')| \mathop{\geq} | Mono(X, H, r')| by hyps$} \\
    \end{flalign}
    $|Mono(X+ F, H, r')| \mathop{\geq} |Mono(X+ F, G, l')|$ :
    $Mono(X, H, r')= Mono(X, G, l')$ and if $h \mathop{\in} Mono(X+ F, G, l')$ then there are two cases:
        \begin{itemize}
            \item if $F$ is in $C$ then $h \mathop{\in} Mono(X+ F, H, r')$
            \item if $F$ is in $L$ then there exists an occurrence of $F$ in $R$ around the same interface elements, thus $h \mathop{\in} Mono(X+ F, H, r')$
            \item otherwise, $F$ is created, since $\rho^{-1}$ is $F$-non-increasing, an occurrence of $F$ is created in $H$ around the same sub-interface, thus $h \mathop{\in} Mono(X+ F, H, r')$
         \end{itemize}
    \todo{debug: les occurrences not around interface elements}
\end{proof}

\begin{proposition}
    $|Mono(X- F, H, \lnot r', \lnot m')| \mathop{\geq} |Mono(X- F, H, \lnot r', m')|$
\end{proposition}
\begin{proof}
    \begin{flalign}
        &|Mono(X- F, G, \lnot l', \lnot m)| - |Mono(X- F, H, \lnot r', \lnot m')| \\
        =&(|Mono(X, G, \lnot l', \lnot m)| - | Mono(X\mathop{+}F, G, \lnot l', \lnot m)|)-\\
        & (|Mono(X, H, \lnot r', \lnot m')| - |Mono(X+ F, H, \lnot r', \lnot m')|) \\
        =&(|Mono(X, G, \lnot l', \lnot m)| - | Mono(X, H, \lnot r', \lnot m')|)\mathop{+}\\
        &(|Mono(X+ F, H, \lnot r', \lnot m')| - |Mono(X+ F, G, \lnot l', \lnot m)|) \\
        \mathop{\geq} &(|Mono(X+ F, H, \lnot r', \lnot m')| - |Mono(X+ F, G, \lnot l', \lnot m)|) 
        \\
        &\text{because $|Mono(X, G, \lnot l', \lnot m)| \mathop{\geq} | Mono(X, H, \lnot r', \lnot m')| by lem$} \\
    \end{flalign}
\end{proof}

\begin{proposition}
    $|Mono(X- F, G, \lnot l', m)| ???? |Mono(X- F, G, \lnot l', \lnot m)|$
\end{proposition}
\begin{proof}
    \begin{flalign}
        &|Mono(X- F, G, \lnot l', m)| - |Mono(X- F, H, \lnot r', m')| \\
        =&(|Mono(X, G, \lnot l', m)| - | Mono(X\mathop{+}F, G, \lnot l', m)|)-\\
        & (|Mono(X, H, \lnot r', m')| - |Mono(X+ F, H, \lnot r', m')|) \\
        =&(|Mono(X, G, \lnot l', m)| - | Mono(X, H, \lnot r', m')|)\mathop{+}\\
            &(|Mono(X+ F, H, \lnot r', m')| - |Mono(X+ F, G, \lnot l', m)|) \\
        =&(|Mono(X, L)| - | Mono(X, R)|)\mathop{+}\\
        &(|Mono(X+ F, H, \lnot r', m')| - |Mono(X+ F, G, \lnot l', m)|) \\
        &\text{by~\autoref{lem:decomp_w_u} and~\autoref{lem:xlnlmxrnr} } \\
    \end{flalign}
    let $h \mathop{\in} Mono(X+ F, G, \lnot l', m)$, then 
    \begin{itemize}
        \item if $F$ is in $C$ then $h \mathop{\in} Mono(X+ F, H, \lnot r', m')$
        \item if $F$ is in $L$ then there exists an occurrence of $F$ in $R$ with ... , thus $h \mathop{\in} Mono(X+ F, H, \lnot r', m')$ \todo{if $F$ is in $L$ then there exists an occurrence of $F$ in $R$ with ... }
        \item otherwise $F$ is created, since $\rho^{-1}$ is $F$-non-increasing, an occurrence of $F$ is created in $H$ around the same sub-interface, thus $h \mathop{\in} Mono(X+ F, H, \lnot r', m')$ \todo{$\rho^{-1}$ is $F$-non-increasing}
    \end{itemize}
\end{proof}
====================================================================================================

\begin{flalign*}
    &\card{Mono(X- \mathbb{F}, G)} - \card{Mono(X- \mathbb{F}, H)} \\
   =&\card{Mono(X- \mathbb{F}, G, l') \uplus Mono(X- \mathbb{F}, G, \lnot l', m) \uplus Mono(X- \mathbb{F}, G, \lnot l', \lnot m)} - \\ 
      &\card{Mono(X- \mathbb{F}, H, r') \uplus Mono(X- \mathbb{F}, G, \lnot r', m') \uplus Mono(X- \mathbb{F}, H, \lnot r', \lnot m')} \\
   =&\left( | Mono(X- \mathbb{F}, G, l')|\mathop{+}|Mono(X- \mathbb{F}, G, \lnot l', m)|+ |Mono(X- \mathbb{F}, G, \lnot l', \lnot m)|\right) - \\ 
    &\left(|Mono(X- \mathbb{F}, H, r')|\mathop{+}|Mono(X- \mathbb{F}, H, \lnot r', m')|\mathop{+}|Mono(X- \mathbb{F}, H, \lnot r', \lnot m')|\right)\\
    \mathop{=} &\left( |Mono(X- \mathbb{F}, G, \lnot l', m)|+ |Mono(X- \mathbb{F}, G, \lnot l', \lnot m)|\right) - \\ 
    &\left(|Mono(X- \mathbb{F}, H, \lnot r', m')|\mathop{+}|Mono(X- \mathbb{F}, H, \lnot r', \lnot m')|\right) \\
    & \text{because $| Mono(X- \mathbb{F}, G, l')| \mathop{=} |Mono(X- \mathbb{F}, H, r')|$} \\
    \mathop{=} &\left( |Mono(X- \mathbb{F}, L)|+ |Mono(X- \mathbb{F}, G, \lnot l', \lnot m)|\right) - \\ 
    &\left(|Mono(X- \mathbb{F}, G, \lnot r', m')|\mathop{+}|Mono(X- \mathbb{F}, H, \lnot r', \lnot m')|\right) \\
    & \text{TODO TODO because $|Mono(X- \mathbb{F}, G, \lnot l', m)| \mathop{=} |Mono(X- \mathbb{F}, L)|$ and $|Mono(X- \mathbb{F}, H, \lnot r', m')| \mathop{=} |Mono(X- \mathbb{F}, R)|$}\\
    \mathop{\geq} &\left( |Mono(X- \mathbb{F}, L)|+ |Mono(X- \mathbb{F}, G, \lnot l', \lnot m)|\right)\\
    & \text{TODO TODO because $|Mono(X- \mathbb{F}, G, \lnot r', m')| \mathop{\geq} |Mono(X- \mathbb{F}, H, \lnot r', \lnot m')|$}
\end{flalign*}


====================================================================================================
\begin{flalign*}
    &\card{Mono(X- \mathbb{F}, G)} - \card{Mono(X- \mathbb{F}, H)} \\
   =&\card{Mono(X, G)\mathop{\setminus} Mono(X+ \mathbb{F}, G)} - \card{Mono(X, H)\mathop{\setminus} Mono(X+ \mathbb{F}, H)} \\
   =&(\card{Mono(X, G)} - \card{Mono(X+ \mathbb{F}, G)}) - (\card{Mono(X, H)} - \card{Mono(X+ \mathbb{F}, H)}) \\
   =&\card{Mono(X, G)} - \card{Mono(X+ \mathbb{F}, G)} - \card{Mono(X, H)}\mathop{+}\card{Mono(X+ \mathbb{F}, H)} \\
   =&(\card{Mono(X, G)} - \card{Mono(X, H)})+(\card{Mono(X+ \mathbb{F}, H)} - \card{Mono(X+ \mathbb{F}, G)}) \\
   \mathop{\geq} & (\card{Mono(X, L)} - \card{Mono(X, R)})+(\card{Mono(X+ \mathbb{F}, H)} - \card{Mono(X+ \mathbb{F}, G)}) & \text{by~\autoref{lem:w_g_geq_w_h_leq}}\\
\end{flalign*}

It suffices, in order to have an approximation of $\card{Mono(X- \mathbb{F}, G)} - \card{Mono(X- \mathbb{F}, H)} $ by analysing $\rho$, to establish a sufficient condition for 
\[\card{Mono(X+ \mathbb{F}, H)} - \card{Mono(X+ \mathbb{F}, G)} \mathop{\geq} 0\]

We have 
\begin{flalign*}
   &\card{Mono(X+ \mathbb{F}, H)} - \card{Mono(X+ \mathbb{F}, G)} 
   \\
   =&\card{Mono(X+ \mathbb{F}, H, r') \uplus Mono(X+ \mathbb{F}, H, \lnot r', m') \uplus  Mono(X+ \mathbb{F}, H, \lnot r', \lnot m') }  - 
   \\ 
   &\card{Mono(X+ \mathbb{F}, G, l') \uplus Mono(X+ \mathbb{F}, G, \lnot l', m) \uplus  Mono(X+ \mathbb{F}, G, \lnot l', \lnot m) } \\
   =&(\card{Mono(X+ \mathbb{F}, H, r')}\mathop{+}\card{Mono(X+ \mathbb{F}, H, \lnot r', m')}\mathop{+}\card{Mono(X+ \mathbb{F}, H, \lnot r', \lnot m') }) - 
   \\  
   &(\card{Mono(X+ \mathbb{F}, G, l')}\mathop{+}\card{Mono(X+ \mathbb{F}, G, \lnot l', m)}\mathop{+}\card{  Mono(X+ \mathbb{F}, G, \lnot l', \lnot m) })
\end{flalign*}

Since $Mono(X+ \mathbb{F}, H, r') \mathop{=} Mono(X+ \mathbb{F}, G, l')$, we have 
\begin{flalign*}
   &\card{Mono(X+ \mathbb{F}, H)} - \card{Mono(X+ \mathbb{F}, G)} \\
   =(&\card{Mono(X+ \mathbb{F}, H, \lnot r', m')}\mathop{+}\card{Mono(X+ \mathbb{F}, H, \lnot r', \lnot m') }) 
   - \\  
   &(\card{Mono(X+ \mathbb{F}, G, \lnot l', m)}\mathop{+}\card{  Mono(X+ \mathbb{F}, G, \lnot l', \lnot m) }) \\
   =&\card{Mono(X+ \mathbb{F}, H, \lnot r', m')}\mathop{+}\card{Mono(X+ \mathbb{F}, H, \lnot r', \lnot m') } 
   - \\  
   &\card{Mono(X+ \mathbb{F}, G, \lnot l', m)} - \card{  Mono(X+ \mathbb{F}, G, \lnot l', \lnot m) } \\ 
   =&(\card{Mono(X+ \mathbb{F}, H, \lnot r', m')} 
    - \card{Mono(X+ \mathbb{F}, G, \lnot l', m)})
   \mathop{+}\\ &(\card{Mono(X+ \mathbb{F}, H, \lnot r', \lnot m') } 
    - \card{  Mono(X+ \mathbb{F}, G, \lnot l', \lnot m) })
\end{flalign*}
If $\card{Mono(X+ \mathbb{F}, H, \lnot r', m')} 
- \card{Mono(X+ \mathbb{F}, G, \lnot l', m)} \mathop{\geq} 0$, which can be calculated precisely, then it suffices to establish a sufficient condition for  \[\card{Mono(X+ \mathbb{F}, H, \lnot r', \lnot m') } 
- \card{  Mono(X+ \mathbb{F}, G, \lnot l', \lnot m) } \mathop{\geq} 0\]
Whic is true by~\autoref{lem:non_decreasing}, if the property defined in Definition~\ref{def:non_decreasing}. Definition~\ref{def:lx} will be needed.